\documentclass[12pt]{article}

\usepackage{amsmath}
\usepackage{amssymb}
\usepackage{graphicx}
\usepackage{tikz}

\counterwithin*{equation}{section}
\counterwithin*{equation}{subsection}
\counterwithin*{equation}{subsubsection}
\addtolength\parskip{\bigskipamount}

\graphicspath{ {./images/} } 

\begin{document}
\section{Chain Rule}
\underline{Recall:} \\
If: \(y=f(x)\) and \(x=g(t)\), then 

\fbox{
	\begin{minipage}{1in}
	\[
		\frac{dy}{dt}=\frac{dy}{dx} * \frac{dx}{dt}
	\]
	\end{minipage}
}

\subsection{Functions of 1 variable}
Consider \(z=f(x,y)\) and \(x=g(t)\) and \(y=h(t)\):\\
\begin{tikzpicture}
	\draw (1.2, 2cm) node[anchor=south west] {z} -- (0, 0) node[anchor=north] {x};
	\draw (1.6, 2cm) -- (2.8, 0) node[anchor=north] {y};
	\draw (2.8, -0.4) -- (2.8,-2.4cm) node[anchor=north] {t};
	\draw (0, -0.4) -- (0,-2.4cm) node[anchor=north] {t};
\end{tikzpicture}

Which depicts \(z=f(x,y)\), \(x=g(t)\), \(y=h(t)\):
\[
	\frac{dz}{dt} = \frac{\partial f}{\partial x} \frac{dx}{dt} + \frac{\partial f}{\partial y} \frac{dy}{dt}
\]
Recall, in order for a function \(z\) to be differentiable at point \((a,b)\), \(\triangle z\) must be able to be put in the form:
\[
	\triangle z = \frac{\partial f}{\partial x} \triangle x + \frac{\partial f}{\partial y} \triangle y + \epsilon_1\triangle x + \epsilon_2\triangle y
\]
Where \(\epsilon_1 \rightarrow 0\) and \(\epsilon_2 \rightarrow 0\) as \((\triangle x, \triangle y) \rightarrow (0,0)\)
If functions \(\epsilon_1\) and \(\epsilon_2\) are not defined at \((0,0)\), we can define them to be 0 there.

Now, we divide both sides of the equation by \(\triangle t\):
\[
	\frac{\triangle z}{\triangle t} = \frac{\partial f}{\partial x} \frac{\triangle x}{\triangle t} + \frac{\partial f}{\partial y} \frac{\triangle y }{\triangle t} + \epsilon_1 \frac{\triangle x}{\triangle t} + \epsilon_2 \frac{\triangle y }{\triangle t}
\]

We show \(\triangle x = g(t+\triangle t) - g(t) \rightarrow 0\) as \(\triangle t \rightarrow 0\), and it is assumed \(g\) is differentiable. 
\\And in the same way, \(\triangle y = h(t+\triangle t) - h(t) \to 0\) as \(\triangle t \to 0\), again assuming \(h\) is differentiable near \(t\).

We know previously from Tangent Planes and Linearization that as \(\triangle x \to 0 \), \(\epsilon_1 \to 0\) and likewise for \(\triangle y\) and \(\epsilon_2\).

Proceeding from there, because \(\epsilon_1 \rightarrow 0\) and \(\epsilon_2 \rightarrow 0\), we can now say:
\begin{align}
	\frac{dz}{dt}=\lim_{\triangle t \to 0} \frac{\triangle z}{\triangle t}
\end{align}
\begin{align}
	= \frac{\partial f}{\partial x} \lim_{\triangle t \to 0} \frac{\triangle x}{\triangle t} + \frac{\partial f}{\partial y} \lim_{\triangle t \to 0} \frac{\triangle y}{\triangle t} + (\lim_{\triangle t \to 0} \epsilon_1)\lim_{\triangle t \to 0} \frac{\triangle x}{\triangle t} + (\lim_{\triangle t \to 0} \epsilon_2) \lim_{\triangle t \to 0} \frac{\triangle y}{\triangle t}
\end{align}
\begin{align}
	= \frac{\partial f}{\partial x} \frac{dx}{dt} + \frac{\partial f}{\partial y} \frac{dy}{dt}+ 0 \cdot \frac{dx}{dt}+0\cdot \frac{dy}{dt}\\
	=\frac{\partial f}{\partial x} \frac{dx}{dt}+ \frac{\partial f}{\partial y} \frac{dy}{dt}
\end{align}
Let us rewrite this for using \(\frac{\partial z}{\partial x} \) instead of \(\frac{\partial f}{\partial x} \):

\fbox{
	\begin{minipage}{1.6in}
		\[
			\frac{dz}{dt} = \frac{\partial z}{\partial x} \frac{dx}{dt} + \frac{\partial z}{\partial y} \frac{dy}{dt}
		\]
	\end{minipage}
}

\subsection{Functions of Multiple Variables}
Now let us look at the case where \(x\) and \(y\) are functions of two variables: \(x = g(s,t)\), \(y=h(s,t)\)

We simply have two differentials rather than a single one:

\noindent\fbox{%
	\begin{minipage}{1.6in}
		\[
			\frac{\partial z}{\partial s} = \frac{\partial f}{\partial x} \frac{dx}{ds}+ \frac{\partial f}{\partial y} \frac{dy}{ds}
		\]
	\end{minipage}	
}
A function of \(t\) 

\noindent\fbox{%
	\begin{minipage}{1.6in}
		\[
			\frac{\partial z}{\partial t} = \frac{\partial f}{\partial x} \frac{dx}{dt}+ \frac{\partial f}{\partial y} \frac{dy}{dt}
		\]
	\end{minipage}	
}
A function of \(s\)

\subsubsection{General Rule}
In general, it can be shown that for \(u=f(x_1,x_2,...,x_n)\), \\%
and \(x_i = g_i(t_1,t_2,...,t_m)\):
\[
	\frac{du}{dt_i} = \sum_{j=1}^{n} \frac{\partial u}{\partial x_j} \cdot \frac{dx_j}{dt_i} = \frac{\partial u}{\partial x_1} \frac{dx}{dt_i} + \frac{\partial u}{\partial x_2}\frac{dx_2}{dt_i} + \hdots + \frac{\partial u}{\partial x_n} \frac{dx_n}{dt_i} 
\].\\
for \(i=1,2,...,m\)
\subsection{Examples}
\subsubsection{Chain Rule Example 1}
If \(z=x^2y^3\), \(x=\cos(2t)\), and \(y=1+\sin t\), then find \(\frac{dz}{dt}\) when \(t=0\).

\subsubsection{Chain Rule Example 2}
Ideal Gas Law \(PV=8.31T\)\\
P = Pressure (kPa)\\
V = volume (L)\\
T = temperature (K)\\
The equation relates these 3 quantities for a mole of an ideal gas. How fast is the volume changing when the temperature is 300K and \underline{increasing} by 0.1K/s, and the pressure is 25kPa and \underline{decreasing} by 0.042 kPa/s?

Givens:\\
\(P = 25kPa\)\\
\(\triangle P = \frac{dP}{dt} = -0.042 kPa/s\)\\
\(T = 300K\)\\
\(\triangle T = \frac{dT}{dt} = 0.1K/s\)\\
\(V = \frac{8.31T}{P}\)

Find \(\frac{dV}{dP}\) and \(\frac{dV}{dT} \).
\begin{align}
	\frac{dV}{dP} = -\frac{8.31T}{P^2}\\
	\frac{dV}{dT} = \frac{8.31}{P}
\end{align}

Now, solve for \(\frac{dV}{dt}\)
\begin{align}
	\frac{dV}{dt} = \frac{\partial V}{\partial P} \frac{dP}{dt} + \frac{\partial V}{\partial T} \frac{dT}{dt}\\
	\frac{dV}{dt} = -\frac{8.31T}{P^2}(-0.042) + \frac{8.31}{P}(0.1)\\
	=\frac{(0.042)(8.31)(300)}{625} + \frac{8.31(0.1)}{25}\\
	\approx .2008
\end{align}
\[
	\therefore \frac{dV}{dt} \approx .2008 L/s
\].

\subsubsection{Chain Rule Example 3}
\(z=e^xcosy\),	\(x=st^3\), \(y=s^3t\)\\
Find \(\frac{dz}{ds}\) and \(\frac{dz}{dt}\).

\subsubsection{Chain Rule Example 4}
\(w=f(x,y,z)\), \(x=x(u,v)\), \(y=y(u,v)\), \(z=z(u,v)\)\\
Find \(\frac{dw}{du}\)

\subsubsection{Chain Rule Example 5}
Suppose \(u=y^4z + x^3z^2\) where \(x=ste^r\), \(y = st^2e^{-r}\), and \(z=s^2t\sin(r)\). \\
Find \(\frac{du}{dt}\) when \(r=0\), \(s=2\), and \(t=1\).

\subsubsection{Chain Rule Example 6}
If \(g(s,t) = f(s^3 - t^3, t^3 - s^3)\), and \(f\) is differentiable, show that g satisfies the equation:
\[
	t^2 \frac{dg}{ds} + s^2 \frac{dg}{dt} = 0
\]
\end{document}
